src/lib/kernel/Kuiper.Kernel.OnlineSoftmax.fsti
@@ -2,53 +2,11 @@ module Kuiper.Kernel.OnlineSoftmax
 
 #lang-pulse
 open Kuiper
-open Kuiper.Seq.Common
-module Vec = Pulse.Lib.Vec
 open Kuiper.Array1
+open Kuiper.Seq.Common
 open Kuiper.Tensor.Layout { ctlayout }
-open Kuiper.Tensor.Layout.Alg { l1_forward }
 
 module SMX = Kuiper.Kernel.Softmax
-
-val max_real: real -> real -> real
-
-let online_softmax_real_iter (md: erased (tuple2 real real)) (x:real) : erased (tuple2 real real) =
-  let (m,d) = md in
-  let m' = max_real m x in
-  let d' = d *. (rexp (m -. m')) +. rexp (x -. m') in
-  (m',d')
-
-let lem_online_softmax_real_iter'
-  (md: erased (tuple2 real real))
-  (x : real)
-  : Lemma (requires snd md >. 0.0R)
-          (ensures snd (online_softmax_real_iter md x) >. 0.0R)
-  = ()
-
-let rec lem_online_softmax_real_iter
-  (init : erased (tuple2 real real))
-  (s : seq real)
-  : Lemma (requires snd init >. 0.0R)
-          (ensures  snd (seq_fold_left #real #(erased (real & real)) online_softmax_real_iter init s) >. 0.0R)
-          (decreases Seq.length s)
-          [SMTPat (seq_fold_left #real #(erased (real & real)) online_softmax_real_iter init s)]
-  = match view_seq s with
-    | SNil -> ()
-    | SCons hd tl -> lem_online_softmax_real_iter (online_softmax_real_iter init hd) tl
-
-let test (x : real { x >. 0.0R }) =
-  assert (x =!= 0.0R)
-
-let online_softmax_real (s:Seq.seq real { Seq.length s > 0 }) : GTot (seq real) =
-  (* TODO: rewrite using some of the stuff in Kuiper.Seq.Common.fsti ?
-  seq_take, seq_drop *)
-  let x = Seq.index s 0 in
-  let (m, (d : real)) = reveal (seq_fold_left online_softmax_real_iter (hide (x, 1.0R)) (seq_drop 1 s)) in
-  // TODO: why ??
-  // assert (d >. 0.0R ==> d =!= 0.0R);
-  // let d': (r: real{r =!= 0.R}) = d in
-  // assert (d =!= 0.0R);
-  seq_map (fun x -> rexp (x -. m) /. d) s
 
 unfold
 type softmax_notinplace_gpu_ty (et : Type0) {| floating et, real_like et, floating_real_like et |} =
@@ -59,7 +17,7 @@ type softmax_notinplace_gpu_ty (et : Type0) {| floating et, real_like et, floati
      (b : array1 et l { is_global b })
      (#va : erased (lseq et lenab))
      (ra : erased (lseq real lenab) { va %~ ra })
-     (#_: squash ( forall (i:natlt lenab). valid (va @! i) /\ min_val `lte` (va @! i)))
+     (#_: squash (seq_forall (fun x -> valid x /\ min_val `lte` x) va))
   preserves
     cpu **
     on gpu_loc (a |-> va)
